[fsub] more

haskell-ref/haskell-system-F/app/Main.hs
@@ -1,0 +1,7 @@
+module Main where
+
+import Test.QuickCheck
+import SystemFClock
+
+main :: IO ()
+main = experiments
