haskell-ref/haskell-system-F/src/SystemFGen.hs
@@ -1,0 +1,364 @@
+{-# LANGUAGE DeriveDataTypeable #-}
+{-# LANGUAGE FlexibleInstances #-}
+{-# LANGUAGE ImplicitParams #-}
+{-# LANGUAGE LambdaCase #-}
+{-# LANGUAGE PartialTypeSignatures #-}
+{-# LANGUAGE ScopedTypeVariables #-}
+{-# OPTIONS_GHC -Wno-missing-methods -Wno-partial-type-signatures #-}
+
+{-
+  Generators and properties for SystemF
+-}
+
+module SystemFGen where
+
+import Control.Monad
+import Control.Monad.State (StateT, evalStateT, get, liftIO, put, runStateT)
+import Data.Data hiding (typeOf)
+import Data.IORef (IORef, modifyIORef, newIORef, readIORef, writeIORef)
+import Data.List
+import qualified Data.Map as M
+import Data.Maybe
+import Data.Ord (comparing)
+import qualified Data.Set as S
+import System.IO.Unsafe (unsafePerformIO)
+import System.Microtimer (formatSeconds, time_)
+import System.Timeout (timeout)
+import SystemF
+import Test.QuickCheck
+import Text.Printf
+
+------------------------------------------
+-- GENERATION
+------------------------------------------
+
+genType :: Int -> Gen Type
+genType freeTypeVar = sized (arb freeTypeVar)
+  where
+    arb ftv 0 = elements $ Base : (TVar <$> [0 .. ftv -1])
+    arb ftv n =
+      oneof
+        [ arb ftv 0,
+          (:->) <$> arb ftv (n `div` 6) <*> arb ftv (n `div` 4),
+          ForAll <$> arb (ftv + 1) (n -1)
+        ]
+
+genExpr :: Gen (Maybe Expr)
+genExpr =
+  sized $ \n -> do t <- genType 0; arb 0 [] t n
+  where
+    arb :: Int -> [Type] -> Type -> Int -> Gen (Maybe Expr)
+    arb ftv c t 0 =
+      oneofMaybe $
+        [return $ Just Con | t == Base]
+          ++
+          -- [ return $ Just BTrue | t == TBool ] ++
+          -- [ return $ Just BFalse | t == TBool ] ++
+          [return $ Just $ Var i | (i, t') <- zip [0 ..] c, t == t']
+          ++ [fmap (Lam t1) <$> arb ftv (t1 : c) t2 0 | (t1 :-> t2) <- [t]]
+          ++ [fmap TLam <$> arb (ftv + 1) (map (liftType 0) c) t1 0 | (ForAll t1) <- [t]]
+    arb ftv c t n =
+      frequency $
+        [(6, arb ftv c t 0)]
+          ++ [(8, fmap (Lam t1) <$> arb ftv (t1 : c) t2 (n -1)) | (t1 :-> t2) <- [t]]
+          ++ [(4, fmap TLam <$> arb (ftv + 1) (map (liftType 0) c) t1 (n -1)) | (ForAll t1) <- [t]]
+          ++ [ ( 8,
+                 do
+                   t2 <- do
+                     arbT <- resize 10 $ genType ftv -- for now; should be bigger?
+                     elements (nub $ michal c t ++ [arbT])
+                   me1 <- arb ftv c (t2 :-> t) (n `div` 2)
+                   me2 <- arb ftv c t2 (n `div` 2)
+                   return $ (:@:) <$> me1 <*> me2
+               )
+             ]
+          ++ [ ( 4,
+                 do
+                   t1t2 <- genT1T2 t
+                   case t1t2 of
+                     Just (t1, t2) -> do
+                       me1 <- arb ftv c t1 (n - 1)
+                       return $ TApp <$> me1 <*> return t2
+                     Nothing -> return Nothing --  ++
+                     -- [ (0, do e1 <- arb ftv c TBool (n `div` 3)
+                     --          e2 <- arb ftv c t (n `div` 3)
+                     --          e3 <- arb ftv c t (n `div` 3)
+                     --          return $ Cond <$> e1 <*> e2 <*> e3) ]
+               )
+             ]
+
+michal :: [Type] -> Type -> [Type]
+michal c t =
+  [ t' | varType <- c, t' <- aux varType ]
+  where
+    aux (t1 :-> t2)
+      | t == t2 = [t1]
+      | t /= t2 = aux t2
+    aux _ = []
+
+-- Check if a type has any type variables.
+-- TODO: replace with "isClosed"
+hasTVars :: Type -> Bool
+hasTVars (TVar _) = True
+hasTVars (t1 :-> t2) = hasTVars t1 || hasTVars t2
+hasTVars (ForAll t) = hasTVars t
+hasTVars TBool = False
+hasTVars Base = False
+
+isClosed :: Type -> Bool
+isClosed = isClosed' 0
+  where
+    isClosed' :: Int -> Type -> Bool
+    isClosed' tc (TVar x) = x < tc
+    isClosed' tc (t1 :-> t2) = isClosed' tc t1 && isClosed' tc t2
+    isClosed' tc (ForAll t) = isClosed' (tc + 1) t
+    isClosed' _ TBool = True
+    isClosed' _ Base = True
+
+-- Randomly fetch a subterm of a type
+fetchSubType :: Type -> Gen (Maybe Type)
+fetchSubType t =
+  oneofMaybe $
+    [return (Just t) | isClosed t]
+      ++ [fetchSubType t1 | (t1 :-> _) <- [t]]
+      ++ [fetchSubType t2 | (_ :-> t2) <- [t]]
+      ++ [fetchSubType t' | (ForAll t') <- [t]]
+
+oneofMaybe :: [Gen (Maybe a)] -> Gen (Maybe a)
+oneofMaybe [] = return Nothing
+oneofMaybe gs = oneof gs
+
+-- "Replace (some occurrences of) closed type s in type t by (TVar n)"
+replaceSubType :: Int -> Type -> Type -> Gen Type
+replaceSubType n s t =
+  oneof $
+    [return t]
+      ++ [return $ TVar n | s == t]
+      ++ [do t1' <- replaceSubType n s t1;
+             t2' <- replaceSubType n s t2;
+             return $ t1' :-> t2' | (t1 :-> t2) <- [t]]
+      ++ [do t'' <- replaceSubType (n + 1) s t';
+             return $ ForAll t'' | (ForAll t') <- [t], t' == s]
+
+-- Generate t1 t2 such that t1{0:=t2} = t
+genT1T2 :: Type -> Gen (Maybe (Type, Type))
+genT1T2 t = do
+  let t' = liftType 0 t
+  t2 <- fetchSubType t'
+  case t2 of
+    Just t2' -> do
+      t1 <- replaceSubType 0 t2' t'
+      return $ Just (ForAll t1, t2')
+    Nothing -> return Nothing
+
+------------------------------------------
+-- SHRINKING
+------------------------------------------
+
+shrinkType :: Type -> [Type]
+shrinkType Base = []
+shrinkType TBool = [Base]
+shrinkType (t1 :-> t2) =
+  Base :
+  t1 :
+  t2 :
+  [t1' :-> t2 | t1' <- shrinkType t1]
+    ++ [t1 :-> t2' | t2' <- shrinkType t2]
+shrinkType (TVar n) = Base : [TVar n' | n' <- shrink n]
+shrinkType (ForAll t) = Base : t : [ForAll t' | t' <- shrinkType t]
+
+shrinkExpr' Con = []
+shrinkExpr' (Var n) = Con : [Var n' | n' <- shrink n]
+shrinkExpr' (Lam t e) =
+  Con :
+  e :
+  [Lam t' e | t' <- shrinkType t]
+    ++ [Lam t e' | e' <- shrinkExpr' e]
+shrinkExpr' (e1 :@: e2) = Con : e1 : e2 : [e1' :@: e2 | e1' <- shrinkExpr' e1] ++ [e1 :@: e2' | e2' <- shrinkExpr' e2]
+shrinkExpr' (Cond e1 e2 e3) = Con : e1 : e2 : e3 : [Cond e1' e2 e3 | e1' <- shrinkExpr' e1] ++ [Cond e1 e2' e3 | e2' <- shrinkExpr' e2] ++ [Cond e1 e2 e3' | e3' <- shrinkExpr' e3]
+shrinkExpr' BTrue = [Con]
+shrinkExpr' BFalse = [Con, BTrue]
+shrinkExpr' (TLam e) = Con : e : [TLam e' | e' <- shrinkExpr' e]
+shrinkExpr' (TApp e t) = Con : e : [TApp e' t | e' <- shrinkExpr' e] ++ [TApp e t' | t' <- shrinkType t]
+
+shrinkExpr :: _ => Expr -> [Expr]
+shrinkExpr e =
+  [e' | e' <- shrinkExpr' e, wellTyped e']
+    ++ [e'' | e' <- shrinkExpr' e, e'' <- shrinkExpr' e', wellTyped e'']
+    ++ [e' | Just e' <- [step e], size e' < size e] --, typeOf e' = typeOf e]
+
+------------------------------------------
+-- PROPERTIES
+------------------------------------------
+
+data PropType
+  = PropStrongNormalization
+  | PropStrongNormalizationStep
+  | PropEvalMakesProgress
+  | PropStepMakesProgress
+  | PropEvalShort
+  | PropBigSmallStep
+  | PropHnfNoStep
+  | PropEvalNoMoreSteps
+  | PropGenWellTyped
+  | PropPreservation
+  | PropParallelPreservation
+  | PropPreservationMulti
+  | PropProgress
+  | PropEvalSame
+  | PropPSame
+  | PropEvalStepSame
+  | PropTest
+  deriving (Show, Read, Eq, Ord, Enum, Bounded, Data, Typeable)
+
+instance Testable (Either String ()) where
+  property (Left s) = whenFail (putStrLn s) False
+  property (Right _) = property True
+
+propOfPropType :: _ => PropType -> (Expr -> Property)
+propOfPropType PropStrongNormalization e = property $ prop_normalform e
+propOfPropType PropStrongNormalizationStep e = property $ prop_normalform' e
+propOfPropType PropEvalMakesProgress e = property $ prop_evalMakesProgress e
+propOfPropType PropStepMakesProgress e = property $ prop_stepMakesProgress e
+propOfPropType PropEvalShort e = property $ prop_evalShort e
+propOfPropType PropBigSmallStep e = property $ prop_bigSmallStep e
+propOfPropType PropHnfNoStep e = property $ prop_hnfNoStep e
+propOfPropType PropEvalNoMoreSteps e = property $ prop_evalNoMoreSteps e
+propOfPropType PropGenWellTyped e = property $ prop_wellTyped e
+propOfPropType PropPreservation e = prop_preservation e
+propOfPropType PropParallelPreservation e = prop_ppreservation e
+propOfPropType PropPreservationMulti e = prop_preservation_multi 0 20 e
+propOfPropType PropProgress e = property $ prop_progress e
+propOfPropType PropEvalSame e = property $ prop_evalSame e
+propOfPropType PropPSame e = property $ prop_PSame e
+propOfPropType PropEvalStepSame e = property $ prop_evalStepSame e
+propOfPropType PropTest e = property $ prop_test e
+
+bToE :: (Show a) => a -> Bool -> Either String ()
+bToE _ True = Right ()
+bToE x False = Left (show x)
+
+prop_normalform e = isHnf . last . eval $ e
+
+prop_normalform' e = isHnf . last . eval' $ e
+
+prop_wellTyped e = wellTyped e
+
+prop_evalMakesProgress e =
+  and (zipWith (/=) es $ drop 1 es)
+  where
+    es = eval e
+
+prop_stepMakesProgress e =
+  and (zipWith (/=) es $ drop 1 es)
+  where
+    es = eval' e
+
+prop_evalShort e =
+  length (eval e) < 100
+
+prop_bigSmallStep e =
+  let es = eval e
+      es' = eval' e
+   in last es == last es'
+
+prop_hnfNoStep e =
+  (not $ isHnf e) || (isNothing $ step e)
+
+prop_evalNoMoreSteps e =
+  isNothing $ step (last $ eval e)
+
+prop_preservation e =
+  case step e of
+    Just s ->
+      whenFail
+        ( do
+            putStrLn $ "Original:  " ++ show e
+            putStrLn $ "With Type: " ++ show (typeOf e)
+            putStrLn $ "Steps To:  " ++ show s
+            putStrLn $ "With Type: " ++ show (typeOf s)
+        )
+        (typeOf e == typeOf s)
+    Nothing -> discard
+
+prop_ppreservation e =
+  let s = pstep e
+   in whenFail
+        ( do
+            putStrLn $ "Original:  " ++ show e
+            putStrLn $ "With Type: " ++ show (typeOf e)
+            putStrLn $ "Steps To:  " ++ show s
+            putStrLn $ "With Type: " ++ show (typeOf s)
+        )
+        (typeOf e == typeOf s)
+
+prop_preservation_multi n max e =
+  if n == max
+    then collect n True
+    else case step e of
+      Just s ->
+        whenFail
+          ( do
+              putStrLn $ "Original:  " ++ show e
+              putStrLn $ "With Type: " ++ show (typeOf e)
+              putStrLn $ "Steps To:  " ++ show s
+              putStrLn $ "With Type: " ++ show (typeOf s)
+          )
+          $ if typeOf e == typeOf s
+            then prop_preservation_multi (n + 1) max s
+            else property False
+      Nothing -> collect n True
+
+prop_progress e = isHnf e || canStep e
+
+prop_evalSame e =
+  take 100 (eval e) == take 100 (eval e)
+
+prop_pevalSame e =
+  (peval e) == peval e
+
+prop_PSame e =
+  (pstep e) == pstep e
+
+prop_evalStepSame e =
+  take 100 (eval' e) == take 100 (eval' e)
+
+prop_test e =
+  case e of
+    (Lam _ (Lam _ _)) :@: (Lam _ _) -> False
+    Lam _ e -> prop_test e
+    TLam e -> prop_test e
+    e1 :@: e2 -> prop_test e1 && prop_test e2
+    TApp e1 _ -> prop_test e1
+    Cond e1 e2 e3 -> prop_test e1 && prop_test e2 && prop_test e3
+    _ -> True
+
+propTimeout :: Int -> (Expr -> Property) -> Maybe Expr -> Property
+propTimeout microseconds p Nothing = discard
+propTimeout microseconds p (Just e) =
+  unsafePerformIO $ do
+    res <- timeout microseconds $ return $! p e
+    case res of
+      Just x -> return x
+      Nothing -> discard
+
+experiments :: IO ()
+experiments = do
+  quickCheckWith stdArgs{maxSuccess=100000} $
+    forAll genExpr $ propTimeout 10000 prop_ppreservation
+--  let t = 100
+--  let setups = Random : [Setup k f | k <- [2], f <- [30]]
+--  let mutants = [SubstInTypeNoDecr]
+--  let time = False
+--  let sep = ";"
+--  let initialCov = M.empty :: M.Map (Description SFC) Int
+-- 
+--  putStrLn . intercalate sep $ "" : (show <$> setups)
+--  forM_ mutants $ \mutant -> do
+--    putStr $ show mutant ++ sep
+--    means <- forM setups $ \setup ->
+--      let ?mutant = mutant
+--       in if time
+--            then formatSeconds . fst <$> trials t (runSetupTime initialCov setup)
+--            else formatMeanCount . fst <$> trials t (runSetupCount initialCov setup)
+--    putStrLn $ intercalate sep means
