haskell-ref/haskell-system-F/ChangeLog.md
@@ -1,0 +1,3 @@
+# Changelog for haskell-system-F
+
+## Unreleased changes
