notes.md
@@ -1,0 +1,71 @@
+# System F <: Benchmark
+
+## Testing (Shifting/Lifting Substitution)
+
+### Subtyping Transitivity 
+
+$$
+\dfrac{\Gamma \vdash S <: T \quad \Gamma \vdash T <: U}{\Gamma \vdash S <: U}
+$$
+
+
+
+### Subtyping Narrowing
+$$
+\dfrac{\Gamma, X <: Q \vdash M <: N \quad \Gamma \vdash P <: Q}{\Gamma, X <: P \vdash M <: N}
+$$
+
+### Subtyping Strengthening 
+
+$$
+\frac{\Gamma, x : Q \vdash S <: T}{\Gamma \vdash S <: T}
+$$
+
+
+##  Generate Typed Terms
+
+### Generate (Concrete) Type Terms
+
+- No terms has exactly type `Top` 
+- Generate `Top` only as the supertype of the parameter in a type abstraction
+
+### Generate Supertype
+
+* Instead of generating terms of subtype, generate supertype based on subtype
+
+
+
+## Testing
+
+### Progress
+
+```coq
+typing empty t U -> value t \/ exists t', t --> t'
+```
+
+### Preservation
+
+```coq
+typing e t U -> red t t' -> typing e t' U
+```
+
+
+
+
+
+
+
+## Verification
+
+### Reduction Semantics 
+
+- `ctx_inj` can be wrong
+- Not sure if it's correct
+- Important to test progress
+- POPLmark required
+- Alternative: Plotkin smallstep / Parallel reduction
+- Alternative: Test Both reduction strategy
+
+### Type Checking
+
+- Stuck! Subtyping correctness requires reasoning on fuel!
